@prefix cs: <http://pid.geoscience.gov.au/def/Access_Codes> .
@prefix dcterms: <http://purl.org/dc/terms/> .
@prefix rdfs: <http://www.w3.org/2000/01/rdf-schema#> .
@prefix sdo: <https://schema.org/> .
@prefix skos: <http://www.w3.org/2004/02/skos/core#> .
@prefix xsd: <http://www.w3.org/2001/XMLSchema#> .

<http://pid.geoscience.gov.au/def/Access_Codes/A> a skos:Concept ;
    rdfs:isDefinedBy cs: ;
    skos:altLabel "A"@en ;
    skos:definition "GA data. This data is restricted to users inside GA. It cannot be released to the public without proper authorisation."@en ;
    skos:inScheme cs: ;
    skos:prefLabel "GA data"@en ;
    skos:topConceptOf cs: .

<http://pid.geoscience.gov.au/def/Access_Codes/C> a skos:Concept ;
    rdfs:isDefinedBy cs: ;
    skos:altLabel "C"@en ;
    skos:definition "Confidential data. A GA security classification. The use of this data is restricted to users with approved access."@en ;
    skos:inScheme cs: ;
    skos:prefLabel "Confidential data"@en ;
    skos:topConceptOf cs: .

<http://pid.geoscience.gov.au/def/Access_Codes/O> a skos:Concept ;
    rdfs:isDefinedBy cs: ;
    skos:altLabel "O"@en ;
    skos:definition "Open data. There are no access restrictions on this data."@en ;
    skos:inScheme cs: ;
    skos:prefLabel "Open data"@en ;
    skos:topConceptOf cs: .

<https://linked.data.gov.au/org/ga/voc-wg> a sdo:Organization ;
    sdo:affiliation <https://linked.data.gov.au/org/ga> ;
    sdo:name "Geoscience Australia Vocabulary Working Group" ;
    sdo:url <https://www.ga.gov.au/data-pubs/datastandards> .

<https://linked.data.gov.au/org/ga> a sdo:Organization ;
    sdo:name "Geoscience Australia" ;
    sdo:url <https://www.ga.gov.au> .

cs: a skos:ConceptScheme ;
    dcterms:created "2019-03-12T11:48:09"^^xsd:dateTime ;
    dcterms:creator <https://linked.data.gov.au/org/ga/voc-wg> ;
    dcterms:modified "2019-03-12T11:48:09"^^xsd:dateTime ;
    dcterms:provenance "GA's ORAPROD database tables"@en ;
    dcterms:publisher <https://linked.data.gov.au/org/ga> ;
    skos:changeNote "This vocabulary created directly from the database"@en ;
    skos:definition "Geoscience Australia's 12-Mar-2019 version of the Access Codes vocabulary"@en ;
    skos:hasTopConcept <http://pid.geoscience.gov.au/def/Access_Codes/A>,
        <http://pid.geoscience.gov.au/def/Access_Codes/C>,
        <http://pid.geoscience.gov.au/def/Access_Codes/O> ;
    skos:prefLabel "Access Codes"@en .